prove function rules

Wasm_Assertions_Shallow.thy
@@ -5,7 +5,7 @@ typedef lvar = "UNIV :: (nat) set" ..
 (* global, local, logical variables*)
 datatype var = Gl nat | Lc nat | Lv lvar
 
-datatype 'a lvar_v = V_p v | V_a 'a
+datatype 'a lvar_v = V_p v | V_n nat | V_a 'a
 
 (* variable store *)
 (* global, local, logical variables*)
@@ -17,11 +17,26 @@ definition var_st_get_local :: "'a var_st \<Rightarrow> nat \<Rightarrow> v opti
                             then Some (st_l!n)
                             else None)"
 
+definition var_st_set_local :: "'a var_st \<Rightarrow> nat \<Rightarrow> v \<Rightarrow> 'a var_st" where
+  "var_st_set_local st n v \<equiv> let (gs, vs, lvs) = st in
+                             (if (n < length vs)
+                             then (gs, vs[n := v], lvs)
+                             else st)"
+
 definition var_st_get_global :: "'a var_st \<Rightarrow> nat \<Rightarrow> global option" where
   "var_st_get_global st n \<equiv> let st_g = (fst st) in
                             (if (n < length st_g)
                             then Some (st_g!n)
                             else None)"
+
+definition var_st_set_global :: "'a var_st \<Rightarrow> nat \<Rightarrow> global \<Rightarrow> 'a var_st" where
+  "var_st_set_global st n g \<equiv> let (gs, vs, lvs) = st in
+                              (if (n < length gs)
+                              then (gs[n := g], vs, lvs)
+                              else st)"
+
+definition var_st_get_lvar :: "'a var_st \<Rightarrow> lvar \<Rightarrow> 'a lvar_v option" where
+  "var_st_get_lvar st lv \<equiv> let st_lv = (snd (snd st)) in st_lv lv"
 
 definition var_st_set_lvar :: "'a var_st \<Rightarrow> lvar \<Rightarrow> 'a lvar_v \<Rightarrow> 'a var_st" where
   "var_st_set_lvar st l lv \<equiv> let (gs, vs, lvs) = st in
@@ -88,13 +103,16 @@ datatype 'a ass = Ass "'a stack_ass" "'a heap_ass" (infix "\<^sub>s|\<^sub>h" 60
 type_synonym 'a triple = "'a ass \<times> e list \<times> 'a ass"
 
 (* function list, assms, label ass, return ass *)
-type_synonym 'a triple_context = "cl list \<times> 'a ass list \<times> 'a ass"
+type_synonym 'a triple_context = "cl list \<times> 'a ass list \<times> 'a ass option"
 
 definition add_label_ass :: "'a triple_context \<Rightarrow> 'a ass \<Rightarrow> 'a triple_context" where
   "add_label_ass \<Gamma> l \<equiv> let (fs, labs, ret) = \<Gamma> in (fs, l#labs, ret)"
 
+definition stack_ass_sat :: "'a stack_ass \<Rightarrow> v list \<Rightarrow> 'a var_st \<Rightarrow> bool" where
+  "stack_ass_sat St ves v_st = list_all2 (\<lambda>Si v. Si v v_st) St ves"
+
 fun ass_sat :: "'a ass \<Rightarrow> v list \<Rightarrow> heap \<Rightarrow> 'a var_st \<Rightarrow> bool" where
-  "ass_sat (St \<^sub>s|\<^sub>h H) ves h st = (list_all2 (\<lambda>Si v. Si v st) St ves \<and> H h st)"
+  "ass_sat (St \<^sub>s|\<^sub>h H) ves h v_st = (stack_ass_sat St ves v_st \<and> H h v_st)"
 | "ass_sat (Ex_ass lv P) ves h st = (\<exists>v. ass_sat P ves h (var_st_set_lvar st lv v))"
 
 fun ass_stack_len :: "'a ass \<Rightarrow> nat" where
@@ -105,75 +123,68 @@ fun ass_stack_len :: "'a ass \<Rightarrow> nat" where
 definition reifies_lab :: "nat list \<Rightarrow> 'a triple_context \<Rightarrow> bool" where
   "reifies_lab lns \<Gamma> \<equiv> lns = map ass_stack_len (fst (snd \<Gamma>))"
 
-(* label reification relation *)
-definition reifies_ret :: "nat \<Rightarrow> 'a triple_context \<Rightarrow> bool" where
-  "reifies_ret rn \<Gamma> \<equiv> rn = ass_stack_len (snd (snd \<Gamma>))"
+(* return reification relation *)
+definition reifies_ret :: "nat option \<Rightarrow> 'a triple_context \<Rightarrow> bool" where
+  "reifies_ret rn \<Gamma> \<equiv> rn = Option.map_option ass_stack_len (snd (snd \<Gamma>))"
+
+locale encapsulated_module =
+fixes i :: inst
+begin
+
+definition ass_wf where
+  "ass_wf lvar_st ret \<Gamma> labs locs s hf st h vcs P \<equiv>
+     ass_sat P vcs h st
+      \<and> heap_disj h hf
+      \<and> reifies_s s i (heap_merge h hf) st (fst \<Gamma>)
+      \<and> reifies_loc locs st
+      \<and> reifies_lab labs \<Gamma>
+      \<and> reifies_ret ret \<Gamma>
+      \<and> snd (snd st) = lvar_st"
+
+definition res_wf where
+  "res_wf \<Gamma> res locs' s' hf vcsf Q \<equiv>
+    let (fs,lasss,rass) = \<Gamma> in
+    (case res of
+       RTrap \<Rightarrow> False
+     | RValue rvs \<Rightarrow> \<exists>h' h'' vcs' st'.
+                             ass_sat Q vcs' h'' st'
+                             \<and> rvs = vcsf@vcs'
+                             \<and> heap_disj h'' hf
+                             \<and> h' = heap_merge h'' hf
+                             \<and> reifies_s s' i h' st' fs
+                             \<and> reifies_loc locs' st'
+     | RBreak n rvs \<Rightarrow> \<exists>h' h'' vcs' st'.
+                             n < length lasss
+                             \<and> ass_sat (lasss!n) vcs' h'' st'
+                             \<and> rvs = vcs'
+                             \<and> heap_disj h'' hf
+                             \<and> h' = heap_merge h'' hf
+                             \<and> reifies_s s' i h' st' fs
+                             \<and> reifies_loc locs' st'
+     | RReturn rvs \<Rightarrow> \<exists>h' h'' vcs' st'.
+                             ass_sat (the rass) vcs' h'' st'
+                             \<and> rvs = vcs'
+                             \<and> heap_disj h'' hf
+                             \<and> h' = heap_merge h'' hf
+                             \<and> reifies_s s' i h' st' fs
+                             \<and> reifies_loc locs' st')"
 
 (* TODO: frame? ? ? ?*)
 definition valid_triple :: "'a triple_context \<Rightarrow> 'a ass \<Rightarrow> e list \<Rightarrow> 'a ass \<Rightarrow> bool" ("_ \<Turnstile> {_}_{_}" 60) where
-  "(\<Gamma> \<Turnstile> {P}es{Q}) \<equiv> let (fs,lasss,rass) = \<Gamma> in
-                     \<forall>vcs h st s i locs labs ret lvar_st.
-                                        ass_sat P vcs h st
-                                      \<and> reifies_s s i h st fs
-                                      \<and> reifies_loc locs st
-                                      \<and> reifies_lab labs \<Gamma>
-                                      \<and> reifies_ret ret \<Gamma>
-                                      \<and> snd (snd st) = lvar_st \<longrightarrow>
-                                      (\<forall>s' locs' res. ((s,locs,($$*vcs)@es) \<Down>{(labs,ret,i)} (s',locs', res)) \<longrightarrow>
-                                      (case res of
-                                         RTrap \<Rightarrow> False
-                                       | RValue rvs \<Rightarrow> \<exists>h' vcs' st'.
-                                                               ass_sat Q vcs' h' st'
-                                                               \<and> rvs = vcs'
-                                                               \<and> reifies_s s' i h' st' fs
-                                                               \<and> reifies_loc locs' st'
-                                       | RBreak n rvs \<Rightarrow> \<exists>h' vcs' st'.
-                                                               n < length lasss
-                                                               \<and> ass_sat (lasss!n) vcs' h' st'
-                                                               \<and> rvs = vcs'
-                                                               \<and> reifies_s s' i h' st' fs
-                                                               \<and> reifies_loc locs' st'
-                                       | RReturn rvs \<Rightarrow> \<exists>h' vcs' st'.
-                                                               ass_sat rass vcs' h' st'
-                                                               \<and> rvs = vcs'
-                                                               \<and> reifies_s s' i h' st' fs
-                                                               \<and> reifies_loc locs' st'))"
+  "(\<Gamma> \<Turnstile> {P}es{Q}) \<equiv> \<forall>vcs h st s locs labs ret lvar_st hf vcsf s' locs' res.
+                                      ((ass_wf lvar_st ret \<Gamma> labs locs s hf st h vcs P \<and>
+                                      ((s,locs,($$*vcsf)@($$*vcs)@es) \<Down>{(labs,ret,i)} (s',locs', res))) \<longrightarrow>
+                                      res_wf \<Gamma> res locs' s' hf vcsf Q)"
 
 definition valid_triples :: "'a triple_context \<Rightarrow> 'a triple set \<Rightarrow> bool" ("_ \<TTurnstile> _" 60) where
   "\<Gamma> \<TTurnstile> specs \<equiv> \<forall>(P,es,Q) \<in> specs. (\<Gamma> \<Turnstile> {P}es{Q})"
 
 (* TODO: frame? ? ? ?*)
 definition valid_triple_n :: "'a triple_context \<Rightarrow> nat \<Rightarrow> 'a ass \<Rightarrow> e list \<Rightarrow> 'a ass \<Rightarrow> bool" ("_ \<Turnstile>'_ _ {_}_{_}" 60) where
-  "(\<Gamma> \<Turnstile>_k {P}es{Q}) \<equiv> let (fs,lasss,rass) = \<Gamma> in
-                     \<forall>vcs h st s i locs labs ret lvar_st.
-                                        ass_sat P vcs h st
-                                      \<and> reifies_s s i h st fs
-                                      \<and> reifies_loc locs st
-                                      \<and> reifies_lab labs \<Gamma>
-                                      \<and> reifies_ret ret \<Gamma>
-                                      \<and> snd (snd st) = lvar_st \<longrightarrow>
-                                      (\<forall>s' locs' res. ((s,locs,($$*vcs)@es)\<Down>k{(labs,ret,i)} (s',locs', res)) \<longrightarrow>
-                                      (case res of
-                                         RTrap \<Rightarrow> False
-                                       | RValue rvs \<Rightarrow> \<exists>h' vcs' st'.
-                                                               ass_sat Q vcs' h' st'
-                                                               \<and> rvs = vcs'
-                                                               \<and> reifies_s s' i h' st' fs
-                                                               \<and> reifies_loc locs' st'
-                                                               \<and> snd (snd st') = lvar_st
-                                       | RBreak n rvs \<Rightarrow> \<exists>h' vcs' st'.
-                                                               n < length lasss
-                                                               \<and> ass_sat (lasss!n) vcs' h' st'
-                                                               \<and> rvs = vcs'
-                                                               \<and> reifies_s s' i h' st' fs
-                                                               \<and> reifies_loc locs' st'
-                                                               \<and> snd (snd st') = lvar_st
-                                       | RReturn rvs \<Rightarrow> \<exists>h' vcs' st'.
-                                                               ass_sat rass vcs' h' st'
-                                                               \<and> rvs = vcs'
-                                                               \<and> reifies_s s' i h' st' fs
-                                                               \<and> reifies_loc locs' st'
-                                                               \<and> snd (snd st') = lvar_st))"
+  "(\<Gamma> \<Turnstile>_k {P}es{Q}) \<equiv> \<forall>vcs h st s locs labs ret lvar_st hf vcsf s' locs' res.
+                                      ((ass_wf lvar_st ret \<Gamma> labs locs s hf st h vcs P \<and>
+                                      ((s,locs,($$*vcsf)@($$*vcs)@es) \<Down>k{(labs,ret,i)} (s',locs', res))) \<longrightarrow>
+                                      res_wf \<Gamma> res locs' s' hf vcsf Q)"
 
 definition valid_triples_n :: "'a triple_context \<Rightarrow> nat \<Rightarrow> 'a triple set \<Rightarrow> bool" ("_ \<TTurnstile>'_ _ _" 60) where
   "(\<Gamma> \<TTurnstile>_n specs) \<equiv> \<forall>(P,es,Q) \<in> specs. (\<Gamma> \<Turnstile>_n {P}es{Q})"
@@ -183,5 +194,67 @@ definition valid_triples_assms :: "'a triple_context \<Rightarrow> 'a triple set
 
 definition valid_triples_assms_n :: "'a triple_context \<Rightarrow> 'a triple set \<Rightarrow> nat \<Rightarrow> 'a triple set \<Rightarrow> bool" ("_\<bullet>_ \<TTurnstile>'_ _ _" 60) where
   "(\<Gamma>\<bullet>assms \<TTurnstile>_n specs) \<equiv> (\<Gamma> \<TTurnstile>_n assms) \<longrightarrow> (\<Gamma> \<TTurnstile>_n specs)"
+
+lemmas valid_triple_defs = valid_triple_def valid_triples_def valid_triples_assms_def
+                           valid_triple_n_def valid_triples_n_def valid_triples_assms_n_def
+
+lemma reifies_func_ind:
+  assumes "reifies_func (funcs s) (inst.funcs i) fs"
+          "j < length fs"
+  shows "sfunc s i j = fs!j"
+  using assms
+  unfolding reifies_func_def
+  by (simp add: list_all2_conv_all_nth sfunc_def sfunc_ind_def)
+
+lemma valid_triples_n_emp: "\<Gamma> \<TTurnstile>_n {}"
+  unfolding valid_triples_n_def
+  by blast
+
+lemma res_wf_conseq:
+  assumes "res_wf \<Gamma> res locs' s' hf vcsf P"
+          "\<forall>vs h vs_t. (ass_sat P vs h vs_t \<longrightarrow> ass_sat P' vs h vs_t)"
+  shows "res_wf \<Gamma> res locs' s' hf vcsf P'"
+  using assms
+  unfolding res_wf_def
+  apply (cases res)
+  apply fastforce+
+  done
+
+lemma ass_wf_conseq:
+  assumes "ass_wf lvar_st ret \<Gamma> labs locs s hf st h vcs P"
+          "\<forall>vs h vs_t. (ass_sat P vs h vs_t \<longrightarrow> ass_sat P' vs h vs_t)"
+  shows "ass_wf lvar_st ret \<Gamma> labs locs s hf st h vcs P'"
+  using assms
+  unfolding ass_wf_def
+  apply fastforce+
+  done
+
+lemma valid_triple_n_conseq:
+  assumes "\<Gamma> \<Turnstile>_n {P'} es {Q'}"
+          "\<forall>vs h vs_t.
+             (ass_sat P vs h vs_t \<longrightarrow>
+              ass_sat P' vs h vs_t) \<and>
+             (ass_sat Q' vs h vs_t \<longrightarrow>
+              ass_sat Q vs h vs_t)"
+  shows "\<Gamma> \<Turnstile>_n {P} es {Q}"
+proof -
+  show ?thesis
+    using assms res_wf_conseq ass_wf_conseq
+    unfolding valid_triple_defs
+    by metis
+qed
+
+lemma valid_triple_assms_n_conseq:
+  assumes "(\<Gamma>\<bullet>assms \<TTurnstile>_n {(P',es,Q')})"
+          "\<forall>vs h vs_t.
+             (ass_sat P vs h vs_t \<longrightarrow>
+              ass_sat P' vs h vs_t) \<and>
+             (ass_sat Q' vs h vs_t \<longrightarrow>
+              ass_sat Q vs h vs_t)"
+  shows "(\<Gamma>\<bullet>assms \<TTurnstile>_n {(P,es,Q)})"
+  using valid_triple_n_conseq[OF _ assms(2)] assms(1)
+  unfolding valid_triples_assms_n_def valid_triples_n_def
+  by simp
+end
 
 end
